refactor to have poly interface

PolyDiv.v
@@ -1,42 +1,19 @@
 Require Import VST.floyd.functional_base.
 Require Import GF2.
-Require Import Poly.
+Require Import PolyDefs.
 (** * A verified, executable version of Euclidean division on polynomials over GF2 *)
 
-(** Monomials *)
-
-(*We provide a special shorthand for the monomial x^n, which will be useful in division*)
-
-Definition monomial (n: nat) :=
-  if Nat.eq_dec n 0%nat then (1 :: nil) else shift (1 :: nil) n.
-
-Lemma monomial_deg: forall n,
-  deg (monomial n) = Z.of_nat n.
-Proof.
-  intros. unfold monomial. if_tac. subst. simpl. reflexivity. rewrite deg_shift. unfold deg. list_solve.
-Qed.
-
-Lemma wf_monomial: forall n,
-  wf_poly (monomial n).
-Proof.
-  intros. unfold monomial. if_tac. unfold wf_poly; intros. reflexivity.
-  unfold shift. unfold wf_poly. intros. rewrite last_last. reflexivity.
-Qed.
-
-Lemma monomial_not_0: forall n,
-  monomial n <> nil.
-Proof.
-  intros. intro. unfold monomial in H. destruct (Nat.eq_dec n 0). inversion H.
-  unfold shift in H. destruct (list_repeat n 0); inversion H.
-Qed.
+(** Note: we define the function in this file as operating on pure lists, then in Poly.v, lift this
+  to polynomials. We do it this way because [poly_div_aux] did not compute when given dependent types as inputs.
+  We have to do the computations on lists, then wrap the outputs in the poly type *)
+Import P.
 
 (** Euclidean Division **)
 
-(*note: may want to make more efficient by shifting instead of add a monomial*)
-Program Fixpoint poly_div_aux (a b q r : poly) (Hb: wf_poly b) (Hr: wf_poly r) {measure (Z.to_nat (deg r + 1))} : 
-  {x: poly * poly | (0<= deg b) ->  wf_poly q ->
-   (deg (snd x) < deg b /\ wf_poly (fst x) /\ wf_poly (snd x) /\
-   (a = poly_add (poly_mult b q) r -> a = poly_add (poly_mult b (fst x)) (snd x)))}
+Program Fixpoint poly_div_aux (a b q r : poly) (Hb: wf_poly b) (Hr: wf_poly r) (Hq: wf_poly q) {measure (Z.to_nat (deg r + 1))} : 
+  {x: { l: poly | wf_poly l} * {l: poly | wf_poly l} |  (b <> nil ->
+   (deg (snd x) < deg b /\ 
+   (a = poly_add (poly_mult b q) r -> a = poly_add (poly_mult b (fst x)) (snd x))))}
   :=
   match b with
   | nil => (nil, nil) (*cannot divide by zero *)
@@ -46,12 +23,11 @@ Program Fixpoint poly_div_aux (a b q r : poly) (Hb: wf_poly b) (Hr: wf_poly r) {
   | right H' => let pow := monomial (Z.to_nat (deg r - deg b)) in
                 let q' := poly_add q pow in
                 let r' := poly_add r (poly_mult b pow) in
-                poly_div_aux a b q' r' Hb (wf_poly_add _ _)
+                poly_div_aux a b q' r' Hb (wf_poly_add _ _) _
   end
 end.
-(*begin hide*)
 Next Obligation.
-lia.
+apply wf_poly_add.
 Defined.
 Next Obligation.
 destruct r.
@@ -78,15 +54,18 @@ apply (poly_add_degree_same (b :: r) (poly_mult (x :: t) (monomial (Z.to_nat (de
 subst. list_solve.
 Defined.
 Next Obligation.
-destruct ((poly_div_aux a (x :: t) (poly_add q (monomial (Z.to_nat (deg r - deg (x :: t)))))
-           (poly_add r (poly_mult (x :: t) (monomial (Z.to_nat (deg r - deg (x :: t)))))) Hb
-           (wf_poly_add r (poly_mult (x :: t) (monomial (Z.to_nat (deg r - deg (x :: t))))))
-           (poly_div_aux_func_obligation_3 (x :: t) r Hb Hr poly_div_aux x t eq_refl H' Heq_anonymous))). simpl.
+destruct  (poly_div_aux a (x :: t) (poly_add q (monomial (Z.to_nat (deg r - deg (x :: t)))))
+                  (poly_add r (poly_mult (x :: t) (monomial (Z.to_nat (deg r - deg (x :: t)))))) Hb
+                  (wf_poly_add r (poly_mult (x :: t) (monomial (Z.to_nat (deg r - deg (x :: t))))))
+                  (poly_div_aux_func_obligation_7 (x :: t) q r Hb x t eq_refl H' Heq_anonymous)
+                  (poly_div_aux_func_obligation_8 (x :: t) r Hb Hr poly_div_aux x t eq_refl H'
+                     Heq_anonymous)). simpl.
 (*in a more workable form - now to prove correctness - ie, that invariant is preserved*)
 destruct x0; simpl in *. 
 assert (wf_poly (poly_add q (monomial (Z.to_nat (deg r - (Zlength (x :: t) - 1)))))).
-apply wf_poly_add. specialize (a0 H H1). destruct a0. destruct H3. destruct H4. split.
-assumption. split. assumption. split. assumption. intros. apply H5. rewrite H6.
+apply wf_poly_add. specialize (a0 H). destruct a0.
+split.
+assumption. intros. apply H2. rewrite H3.
 remember (x :: t) as b.
 remember  (monomial (Z.to_nat (deg r - (Zlength b - 1)))) as pow.
 rewrite poly_mult_distr_l.
@@ -94,97 +73,3 @@ symmetry. rewrite poly_add_assoc. f_equal. rewrite poly_add_comm.
 rewrite poly_add_assoc. rewrite poly_add_inv. rewrite poly_add_comm. apply poly_add_id. apply Hr.
 assumption. assumption. subst. apply wf_monomial.
 Defined.
-(*end hide*)
-
-Definition poly_div a b (Ha: wf_poly a) (Hb : wf_poly b) : poly * poly :=
-  proj1_sig (poly_div_aux a b nil a Hb Ha).
-
-(*begin hide*)
-
-Definition testa := (1 :: 1 :: 0 :: 1 :: nil).
-Lemma wf_a : wf_poly testa.
-Proof.
-unfold wf_poly. unfold testa. simpl. intros. reflexivity.
-Qed.
-
-Definition testb := (1 :: 1 :: nil).
-Lemma wf_b : wf_poly testb.
-Proof.
-  unfold wf_poly. unfold testb. simpl. reflexivity.
-Qed.
-
-Eval compute in (poly_add(poly_mult (0 :: 1 :: 1 :: nil) (1 :: 1 :: nil)) (1 :: nil)).
-Eval compute in ( poly_div testa testb wf_a wf_b  ).
-(*it works!*)
-(*end hide*)
-Section DivFacts.
-
-Lemma remainder_unique: forall a b q1 r1 q2 r2,
-  wf_poly a ->
-  wf_poly b ->
-  wf_poly q1 ->
-  wf_poly r1 ->
-  wf_poly q2 ->
-  wf_poly r2 ->
-  b <> nil ->
-  deg r1 < deg b ->
-  deg r2 < deg b ->
-  a = poly_add (poly_mult q1 b) r1 ->
-  a = poly_add (poly_mult q2 b) r2 ->
-  q1 = q2 /\ r1 = r2.
-Proof.
-  intros. subst. rewrite poly_add_comm in H9. rewrite poly_add_cancel_1 in H9. symmetry in H9.
-  rewrite <- poly_add_assoc in H9.
-  rewrite poly_add_cancel_1 in H9.
-  assert (deg (poly_add r2 r1) = deg (poly_add (poly_mult q1 b) (poly_mult q2 b))). rewrite H9; reflexivity.
-  pose proof (poly_add_degree_max r2 r1).
-  rewrite <- poly_mult_distr_r in H8.
-  destruct (poly_add q1 q2) eqn : P. all: try assumption. all: try (apply wf_poly_add).
-  - rewrite poly_add_inv_iff in P; try assumption. subst. 
-    rewrite poly_mult_0_l in H8. simpl in H8.
-    destruct (poly_add r2 r1) eqn : R. rewrite poly_add_inv_iff in R; try assumption. auto.
-    simpl in H8. list_solve.
-  - rewrite <- P in H8. rewrite poly_mult_deg in H8.
-    assert (deg (poly_add q1 q2) < 0) by lia.
-    assert (poly_add q1 q2 = nil). destruct (poly_add q1 q2). reflexivity. simpl in H11.
-    list_solve. rewrite poly_add_inv_iff in H12. subst.
-    rewrite poly_add_inv in H9. symmetry in H9. rewrite poly_add_inv_iff in H9. subst. auto.
-    all: try assumption. all: try(apply wf_poly_add). intro. rewrite P in H11. inversion H11.
-Qed.
-
-Lemma poly_div_wf: forall a b q r (Ha: wf_poly a) (Hb: wf_poly b),
-  b <> nil ->
-  poly_div a b Ha Hb = (q,r) ->
-  wf_poly q /\ wf_poly r.
-Proof.
-  intros. unfold poly_div in H0. destruct  (poly_div_aux a b nil a Hb Ha).
-  simpl in H0. destruct x; subst. simpl in a0. inversion H0; subst. split. apply a0.
-  unfold deg. destruct b. contradiction. list_solve. apply wf_poly_nil.
-  apply a0. destruct b; simpl. contradiction. list_solve. apply wf_poly_nil.
-Qed. 
-  
- 
-Lemma poly_div_correct: forall a b q r (Ha: wf_poly a) (Hb : wf_poly b),
-  wf_poly q ->
-  wf_poly r ->
-  b <> nil ->
-  deg r < deg b ->
-  poly_div a b Ha Hb = (q,r) <-> a = poly_add (poly_mult q b) r.
-Proof.
-  intros. split; intros.
-  - unfold poly_div in H3. destruct (poly_div_aux a b nil a Hb Ha). simpl in H3.
-    destruct x; inversion H3; subst; simpl in *. clear H3.
-    assert (deg r < deg b /\ wf_poly q /\ wf_poly r /\ (a = poly_add nil a -> a = poly_add (poly_mult b q) r)).
-    apply a0. destruct b; simpl. contradiction. list_solve. apply wf_poly_nil. clear a0.
-    rewrite poly_mult_comm;try apply H3. symmetry. apply poly_add_id. all: assumption.
-  - unfold poly_div. destruct (poly_div_aux a b nil a Hb Ha). simpl. destruct x; simpl in *.
-    assert (deg p0 < deg b /\
-     wf_poly p /\ wf_poly p0 /\ (a = poly_add nil a -> a = poly_add (poly_mult b p) p0)).
-    apply a0. destruct b; simpl. contradiction. list_solve. apply wf_poly_nil. clear a0.
-    destruct H4. destruct H5. destruct H6.
-    assert (p = q /\ p0 = r). eapply remainder_unique. apply Ha. apply Hb. 
-    all: try assumption. rewrite poly_mult_comm; try assumption. apply H7.
-    symmetry. apply poly_add_id. assumption. destruct H8; subst. reflexivity.
-Qed.  
-    
-End DivFacts.
